new/proof/github_com/goose_lang/goose/testdata/examples/semantics.v
@@ -142,4 +142,16 @@ Proof.
   (* TODO: looks like translation bug *)
 Abort.
 
+(* this doesn't formally mean much but if panic is opaque it tells you the code
+has a panic *)
+Lemma wp_shouldPanic :
+  ∀ (Φ: goose_lang.val → iProp Σ),
+  (∀ Ψ (v: goose_lang.val), WP @! go.panic v {{ Ψ }}) -∗
+  WP @! semantics.shouldPanic #() {{ Φ }}.
+Proof.
+  iIntros (Φ) "Hpanic".
+  wp_func_call. wp_call.
+  wp_apply "Hpanic".
+Qed.
+
 End wps.
